src/QueryStructure/Implementation/DataStructures/BagADT/BagADT.v
@@ -17,43 +17,51 @@ Section BagADT.
   Variable MatchSearchTerm : SearchTermType -> ElementType -> bool.
   Variable ApplyUpdateTerm : UpdateTermType -> ElementType -> ElementType.
 
+  Definition sEmpty := "Empty".
+  Definition sFind := "Find".
+  Definition sEnumerate := "Enumerate".
+  Definition sInsert := "Insert".
+  Definition sCount := "Count".
+  Definition sDelete := "Delete".
+  Definition sUpdate := "Update".
+
   (* Get rid of Bag. *)
   Definition BagSig : ADTSig :=
     ADTsignature {
-        Constructor "Empty" : unit             -> rep,
-        Method "Find"      : rep x SearchTermType -> rep x list ElementType,
-        Method "Enumerate" : rep x unit -> rep x list ElementType,
-        Method "Insert"    : rep x ElementType -> rep x unit,
-        Method "Count"     : rep x SearchTermType  -> rep x nat,
-        Method "Delete"    : rep x SearchTermType  -> rep x (list ElementType),
-        Method "Update"    : rep x (SearchTermType * UpdateTermType) -> rep x (list ElementType)
+        Constructor sEmpty : unit             -> rep,
+        Method sFind      : rep x SearchTermType -> rep x list ElementType,
+        Method sEnumerate : rep x unit -> rep x list ElementType,
+        Method sInsert    : rep x ElementType -> rep x unit,
+        Method sCount     : rep x SearchTermType  -> rep x nat,
+        Method sDelete    : rep x SearchTermType  -> rep x (list ElementType),
+        Method sUpdate    : rep x (SearchTermType * UpdateTermType) -> rep x (list ElementType)
   }.
 
   Definition BagSpec : ADT BagSig :=
     ADTRep (IndexedEnsemble) {
-        Def Constructor "Empty" (_ : unit) : rep :=
+        Def Constructor sEmpty (_ : unit) : rep :=
           ret (Empty_set _),
 
-        Def Method "Find" (r : rep, f : SearchTermType)
+        Def Method sFind (r : rep, f : SearchTermType)
           : list ElementType :=
             results <- {l | EnsembleIndexedListEquivalence r l};
             ret (r, filter (MatchSearchTerm f) results),
 
-        Def Method "Enumerate" (r : rep, f : unit)
+        Def Method sEnumerate (r : rep, f : unit)
           : list ElementType :=
             results <- {l | EnsembleIndexedListEquivalence r l};
             ret (r, results),
 
-        Def Method "Insert" (r : rep, element : ElementType) : unit :=
+        Def Method sInsert (r : rep, element : ElementType) : unit :=
           freshIdx <- {freshIdx | UnConstrFreshIdx r freshIdx};
           ret (Add _ r {| elementIndex := freshIdx;
                           indexedElement := element |}, ()),
 
-        Def Method "Count" (r : rep, f : SearchTermType) : nat :=
+        Def Method sCount (r : rep, f : SearchTermType) : nat :=
           results <- {l | EnsembleIndexedListEquivalence r l};
         ret (r, length (filter (MatchSearchTerm f) results)),
 
-        Def Method "Delete" (r : rep, f : SearchTermType)
+        Def Method sDelete (r : rep, f : SearchTermType)
         : list ElementType :=
           deleted <- {l | EnsembleIndexedListEquivalence r l};
           ret (EnsembleDelete
@@ -61,7 +69,7 @@ Section BagADT.
                  (fun tup => MatchSearchTerm f tup = true),
                filter (MatchSearchTerm f) deleted),
 
-        Def Method "Update" (r : rep, f : SearchTermType * UpdateTermType) : list ElementType :=
+        Def Method sUpdate (r : rep, f : SearchTermType * UpdateTermType) : list ElementType :=
             updated <- {l | EnsembleIndexedListEquivalence r l};
             ret (IndexedEnsembleUpdate r (fun tup => MatchSearchTerm (fst f) tup = true) (ApplyUpdateTerm (snd f)),
                  filter (MatchSearchTerm (fst f)) updated)
